Finished the completeness proof for existential Hoare logic.
Gave up on dealing with dependent type and impredicativity hell, and defined ceval as Type.

theories/EHoare.v
@@ -15,14 +15,14 @@ Definition ehoare_triple
            (P : Assertion) (c : com) (Q : Assertion) : Prop :=
   forall st,
      P st ->
-     exists st', st =[ c ]=> st' /\ Q st'.
+     exists st' (exe : st =[ c ]=> st'), Q st'.
 
 Notation "{{ P }}  c  {{ Q }}#" :=
   (ehoare_triple P c Q) (at level 90, c at next level)
   : hoare_spec_scope.
 
 Definition ewp (c:com) (Q:Assertion) : Assertion :=
-  fun st => exists st', st =[ c ]=> st' /\ Q st'.
+  fun st => exists st' (exe : st =[ c ]=> st'), Q st'.
 
 Lemma ewp_is_precondition: forall c Q,
   {{ewp c Q}} c {{Q}}#.
@@ -87,7 +87,7 @@ Proof.
   - edestruct H; eauto. destruct_conjs.
     edestruct IH; eauto. destruct_conjs.
     eauto.
-  - firstorder with hoare.
+  - repeat econstructor; eauto. firstorder with hoare.
 Qed.
 
 Theorem ehoare_proof_sound : forall P c Q,
@@ -105,7 +105,9 @@ Proof.
   - (* ;; *)
     firstorder eauto.
   - (* TEST *)
-    destruct (beval st b) eqn:?; firstorder with hoare.
+    destruct (beval st b) eqn:?.
+    + edestruct IHpf1; firstorder eauto.
+    + edestruct IHpf2; firstorder eauto. firstorder with hoare.
   - (* WHILE *)
     eapply ehoare_while; eauto.
   - (* Conseq *)
@@ -113,41 +115,45 @@ Proof.
 Qed.
 
 Inductive loop_sizeR : forall {st c st'}, st =[ c ]=> st' -> nat -> Prop :=
-| LS_WhileFalse : forall b st c pff,
-    loop_sizeR (E_WhileFalse b st c pff) 0
-| LS_WhileTrue : forall st st' st'' b c pft pfc pfw n,
-    loop_sizeR pfw n ->
-    loop_sizeR (E_WhileTrue st st' st'' b c pft pfc pfw) (S n)
+| LS_WhileFalse : forall b st c exef,
+    loop_sizeR (E_WhileFalse b st c exef) 0
+| LS_WhileTrue : forall st st' st'' b c pft exec exew n,
+    loop_sizeR exew n ->
+    loop_sizeR (E_WhileTrue st st' st'' b c pft exec exew) (S n)
 .
 
 Definition loop_measureR b c (Q : Assertion)
            (st : state) (n : nat) : Prop :=
-  (~ (exists st', st =[ WHILE b DO c END ]=> st' /\ Q st') -> n = 0) /\
-  (forall m st' (pf : st =[ WHILE b DO c END ]=> st'),
+  (~ (exists st' (exe : st =[ WHILE b DO c END ]=> st'), Q st') -> n = 0) /\
+  (forall m st' (exe : st =[ WHILE b DO c END ]=> st'),
       Q st' ->
-      loop_sizeR pf m ->
-      (forall m' st'' (pf' : st =[ WHILE b DO c END ]=> st''),
+      loop_sizeR exe m ->
+      (forall m' st'' (exe' : st =[ WHILE b DO c END ]=> st''),
           Q st'' ->
-          loop_sizeR pf' m' ->
+          loop_sizeR exe' m' ->
           m <= m') ->
       n = m).
 
-Scheme ceval_ind_dep := Induction for ceval Sort Prop.
-
-Lemma loop_sizeR_ex : forall st b c st' (pf : st =[ WHILE b DO c END ]=> st'),
-    exists n, loop_sizeR pf n.
+Lemma loop_sizeR_ex : forall st b c st' (exe : st =[ WHILE b DO c END ]=> st'),
+    exists n, loop_sizeR exe n.
 Proof.
   intros. remember (WHILE b DO c END)%imp as c' eqn:Heq.
-  induction pf using ceval_ind_dep; inversion Heq; subst.
+  induction exe; inversion Heq; subst.
   - repeat econstructor.
-  - destruct IHpf2; auto. repeat econstructor. eauto.
+  - firstorder eauto. repeat econstructor. eauto.
 Qed.
 
 Lemma loop_sizeR_inv : forall st st' st'' b c pft pfc pfw n,
     loop_sizeR (E_WhileTrue st st' st'' b c pft pfc pfw) n ->
     exists m, loop_sizeR pfw m /\ S m = n.
 Proof.
-  Admitted.
+  intros until n. inversion 1.
+  repeat match goal with
+         | H : existT _ _ _ = existT _ _ _ |- _ =>
+           apply inj_pair2 in H; subst
+         end.
+  eauto.
+Qed.
 
 Lemma nonempty_smallest_ex (P : nat -> Prop) :
   (exists n, P n) ->
@@ -160,17 +166,17 @@ Proof.
 Qed.
 
 Lemma loop_measureR_ex b c Q st :
-  (exists st', st =[ WHILE b DO c END ]=> st' /\ Q st') ->
-  exists m st' (pf : st =[ WHILE b DO c END ]=> st'),
-    Q st' /\ loop_sizeR pf m /\
-    (forall m' st'' (pf' : st =[ WHILE b DO c END ]=> st''),
-        Q st'' -> loop_sizeR pf' m' -> m <= m').
+  (exists st' (exe : st =[ WHILE b DO c END ]=> st'), Q st') ->
+  exists m st' (exe : st =[ WHILE b DO c END ]=> st'),
+    Q st' /\ loop_sizeR exe m /\
+    (forall m' st'' (exe' : st =[ WHILE b DO c END ]=> st''),
+        Q st'' -> loop_sizeR exe' m' -> m <= m').
 Proof.
   intros.
   edestruct (nonempty_smallest_ex
-               (fun m => exists st' (pf : st =[ WHILE b DO c END ]=> st'),
-                    Q st' /\ loop_sizeR pf m)) as [m ?].
-  - destruct H as [? [H ?]]. edestruct loop_sizeR_ex with (pf:=H). eauto.
+               (fun m => exists st' (exe : st =[ WHILE b DO c END ]=> st'),
+                    Q st' /\ loop_sizeR exe m)) as [m ?].
+  - destruct H as [? [H ?]]. edestruct loop_sizeR_ex with (exe:=H). eauto.
   - destruct_conjs. exists m. repeat econstructor; eauto.
 Qed.
 
@@ -178,8 +184,8 @@ Lemma loop_measureR_is_fun b c Q : forall (st : state),
     exists! n, loop_measureR b c Q st n.
 Proof.
   unfold unique.
-  intros. destruct (classic (exists st', st =[ WHILE b DO c END ]=> st' /\ Q st')) as [H | H].
-  - apply loop_measureR_ex in H. destruct H as [m [st' [pf ?]]]. destruct_conjs.
+  intros. destruct (classic (exists st' (exe : st =[ WHILE b DO c END ]=> st'), Q st')) as [H | H].
+  - apply loop_measureR_ex in H. destruct H as [m ?]. destruct_conjs.
     exists m. split.
     + split. intros. exfalso. eauto.
       intros m'. intros. assert (m <= m') by eauto. assert (m' <= m) by eauto.
@@ -192,12 +198,12 @@ Proof.
       symmetry. eauto.
 Qed.
 
-Lemma loop_measureR_order : forall (Q : Assertion) st st' st'' b c pft pfc pfw m,
+Lemma loop_measureR_order : forall (Q : Assertion) st st' st'' b c pft exec exew m,
     Q st'' ->
-    loop_sizeR (E_WhileTrue st st' st'' b c pft pfc pfw) m ->
-    (forall m' st''' (pf' : st =[ WHILE b DO c END ]=> st'''),
+    loop_sizeR (E_WhileTrue st st' st'' b c pft exec exew) m ->
+    (forall m' st''' (exe' : st =[ WHILE b DO c END ]=> st'''),
         Q st''' ->
-        loop_sizeR pf' m' ->
+        loop_sizeR exe' m' ->
         m <= m') ->
     forall m', loop_measureR b c Q st' m' ->
           S m' = m.
@@ -219,45 +225,45 @@ Proof.
   induction c; intros P Q HT.
   - (* SKIP *)
     eapply EH_Consequence; eauto with hoare.
-    intros. edestruct HT as [? [HE ?]]; eauto.
-    inversion HE; subst. eauto.
+    intros. edestruct HT as [? [exe ?]]; eauto.
+    inversion exe; subst. eauto.
   - (* ::= *)
     eapply EH_Consequence; eauto with hoare.
-    intros. edestruct HT as [? [HE ?]]; eauto.
-    inversion HE; subst. eauto.
+    intros. edestruct HT as [? [exe ?]]; eauto.
+    inversion exe; subst. eauto.
   - (* :::= *)
     eapply EH_Consequence; eauto with hoare.
-    simpl. intros. edestruct HT as [? [HE ?]]; eauto.
-    inversion HE; subst. eauto.
+    simpl. intros. edestruct HT as [? [exe ?]]; eauto.
+    inversion exe; subst. eauto.
   - (* ;; *)
     apply EH_Seq with (ewp c2 Q); eauto. apply IHc1.
-    intros. edestruct HT as [? [HE ?]]; eauto.
-    inversion HE; subst. firstorder.
+    intros. edestruct HT as [? [exe ?]]; eauto.
+    inversion exe; subst. repeat econstructor; eauto.
   - (* IFB *)
     apply EH_If.
     + apply IHc1. intros. destruct_conjs.
-      edestruct HT as [? [HE ?]]; eauto.
-      inversion HE; subst; firstorder with hoare.
+      edestruct HT as [? [exe ?]]; eauto.
+      inversion exe; subst; firstorder with hoare.
     + apply IHc2. intros. destruct_conjs.
-      edestruct HT as [? [HE ?]]; eauto.
-      inversion HE; subst; firstorder with hoare.
+      edestruct HT as [? [exe ?]]; eauto.
+      inversion exe; subst; firstorder with hoare.
   - (* WHILE *)
     eapply EH_Consequence with (P':=ewp (WHILE b DO c END) Q).
     + destruct (unique_choice _ _
                               (loop_measureR b c Q)
                               (loop_measureR_is_fun b c Q)) as [measure Hm].
       apply EH_While with (E:=measure).
-      intros. apply IHc. intros ? [Hwp ?]. destruct_conjs. subst.
+      intros. apply IHc. intros. destruct_conjs. subst.
       destruct (Hm st) as [_ Hm'].
-      edestruct loop_measureR_ex as [m [st' [pf ?]]]; eauto. destruct_conjs.
+      edestruct loop_measureR_ex as [m [st' [exe ?]]]; eauto. destruct_conjs.
       remember (WHILE b DO c END)%imp eqn:Heq.
-      destruct pf; inversion Heq; subst; clear Heq. exfalso. congruence.
-      eexists. intuition eauto.
+      destruct exe; inversion Heq; subst; clear Heq. exfalso. congruence.
+      exists st'. eexists; eauto. intuition eauto.
       eapply loop_measureR_order in Hm; eauto.
       assert (measure st = m) by eauto. lia.
     + eauto.
-    + simpl. intros ? [H ?]. destruct H as [? [H ?]].
-      inversion H; subst; eauto. exfalso. eauto.
+    + simpl. intros ? [H ?]. destruct H as [? [exe ?]].
+      inversion exe; subst; eauto. exfalso. eauto.
 Qed.
 
 End EHoare.
